Updated model to using global variable for memory and reverts

src/YulPrimops.ec
@@ -7,23 +7,23 @@ op calldata : uint256 array.
 (* op keccak256 : uint256 array -> uint256. *)
 
 module Primops = {
-  var m : mem
+  var memory : mem
+  var reverted : bool
 
   proc mload(a : uint256) : uint256 = {
-    return m.[a];
+    return memory.[a];
   }
 
   proc mstore(a : uint256, v : uint256): unit = {
-    m <- m.[a<-v];
+    memory <- memory.[a<-v];
   }
 
-  proc mstore8(a : uint256, v : uint256) : uint256 = {
+  proc mstore8(a : uint256, v : uint256) : unit = {
     (* TODO: memory model? *)
-    return m.[a];
   }
 
   proc ret(retOff : uint256, retSize : uint256) : unit = {
-    (* TODO: Implement return, needs to be differentiable from revert *)
+    (* TODO: Implement return *)
     return ();
   }
 
@@ -55,44 +55,37 @@ module Primops = {
     return W256.zero;
   }
 
-  proc staticcall(gas : uint256, addr : uint256, argOff : uint256, argSize : uint256, retOff : uint256, retSize : uint256, m : mem) : uint256 * mem = {
-    var succ, m';
+  proc staticcall(gas : uint256, addr : uint256, argOff : uint256, argSize : uint256, retOff : uint256, retSize : uint256) : uint256 = {
+    var succ;
     if (addr = W256.of_int 5) {
       (* TODO: modexp *)
       succ <- W256.zero;
-      m' <- m;
     } else {
       if (addr = W256.of_int 6) {
         (* TODO: ecAdd *)
         succ <- W256.zero;
-        m' <- m;
       } else {
         if (addr = W256.of_int 7) {
           (* TODO: ecMul *)
           succ <- W256.zero;
-          m' <- m;
         } else {
           if (addr = W256.of_int 8) {
             (* TODO: ecPairing *)
             succ <- W256.zero;
-            m' <- m;
           } else {
               succ <- W256.zero;
-              m' <- m;
           }
         }
       }
     }
-    return (succ, m');
+    return succ;
   }
 
   proc revert() : unit = {
-    (* TODO: Implement revert, needs to be differentiable from return *)
-    return ();
+    reverted <- true;
   }
 
   proc calldataload(i : uint256) : uint256 = {
-    (* Needs a fix, for some reason the _.[_] notation no longer works once JWord is included as a depency (In UInt256.ec) *) 
     return calldata.[W256.to_uint i];
   }
 }.
